+++
title = '3.333'
translationKey = '3.333'
date = 2023-11-26T13:02:22+01:00
draft = false
+++

A function cannot be its own argument, because the functional sign already contains the prototype of its own argument and it cannot contain itself.
If, for example, we suppose that the function <span class="mathmode"><var>F</var>(<var>fx</var>)</span> could be its own argument, then there would be a proposition “<span class="mathmode"><var>F</var>(<var>F</var>(<var>fx</var>))</span>”, and in this the outer function <span class="mathmode"><var>F</var></span> and the inner function <span class="mathmode"><var>F</var></span> must have different meanings; for the inner has the form <span class="mathmode"><var>φ</var>(<var>fx</var>)</span>, the outer the form <span class="mathmode"><var>ψ</var>(<var>φ</var>(<var>fx</var>))</span>. Common to both functions is only the letter “<span class="mathmode"><var>F</var></span>”, which by itself signifies nothing.
This is at once clear, if instead of “<span class="mathmode"><var>F</var>(<var>Fu</var>)</span>” we write “<span class="mathmode"><span class="quant">(<span class="symbol">∃</span><var>φ</var>):</span><var>F</var>(<var>φu</var>)<span class="mathrel">.</span><var>φu</var><span class="mathrel">=</span><var>Fu</var></span>”.
Herewith Russell’s paradox vanishes.
